# core ontologies of the cellograph project
@prefix : <http://www.spatialai.org/CelloGraph/v1.0/core.owl#>  . 
@prefix cg: <http://www.spatialai.org/CelloGraph/v1.0/core.owl#>  . 
#@prefix cg-bonds: <http://www.spatialai.org/CelloGraph/v1.0/chemicalbonds.owl#>  . 
@prefix sp: <http://www.spatialai.org/SciPub/v1.0/>  .

# reused ontologies
@prefix bfo:  <http://purl.obolibrary.org/obo/bfo.owl#> . 
@prefix chebi: <http://purl.obolibrary.org/obo/chebi.owl#> . 
@prefix iof: <https://purl.industrialontologies.org/ontology/core/20220506/Core/> . 

# generic prefixes
@prefix rdf: <http://www.w3.org/1999/02/22-rdf-syntax-ns#> .
@prefix rdfs: <http://www.w3.org/2000/01/rdf-schema#> .
@prefix xml: <http://www.w3.org/XML/1998/namespace> .
@prefix xsd: <http://www.w3.org/2001/XMLSchema#> .
@prefix owl: <http://www.w3.org/2002/07/owl#> .
@prefix dcterms: <http://purl.org/dc/terms/> .
@prefix skos: <http://www.w3.org/2004/02/skos/core#> .
# wordnet and related ontologies
@prefix wn: <http://wordnet-rdf.princeton.edu/ontology#> .
@prefix pwnid: <http://wordnet-rdf.princeton.edu/id/> .
@prefix ontolex: <http://www.w3.org/ns/lemon/ontolex#> .

@base <http://www.spatialai.org/CelloGraph/v1.0/chemicalbonds.owl#> .


<http://www.spatialai.org/CelloGraph/v1.0/chemicalbonds.owl#> rdf:type  owl:Ontology ;
        owl:versionIRI <http://www.spatialai.org/CelloGraph/v1.0/> ;
        rdfs:label         "Chemical Bonds Module of the CelloGraph Ontology"@en-US ;
		dcterms:title "Chemical Bonds Module of the CelloGraph Ontology"@en-US ;
        dcterms:description "The module that describes chemical bonds of the Cellograph Ontology."@en-US ;
        dcterms:created    "2023-01-27"^^xsd:Date ;
        dcterms:creator <http://orcid.org/0000-0002-5331-5052> ;
        dcterms:creator    "Torsten Hahmann"@en-US ;
		dcterms:modified   "2023-01-27"^^xsd:Date ;
        dcterms:issued 	   "2023-01-27"^^xsd:date ;
        dcterms:publisher  <http://spatialai.org/> ;
        dcterms:rights     "Copyright 2023 UMaine, SKAI Lab."@en-US ;
        dcterms:subject    "Ontology"@en-US ;
        owl:versionIRI     <http://www.spatialai.org/CelloGraph/v1.0/chemicalbonds.owl#> ;
        owl:versionInfo    "1.0"@en-US ;
		dcterms:source "https://github.com/thahmann/CelloGraph/ontologies/cellograph/v1.0/chemicalbonds.owl"^^<xsd:anyURI> ;
		owl:imports "https://github.com/thahmann/CelloGraph/ontologies/cellograph/v1.0/core.owl".

# BFO occurrent
###  http://purl.obolibrary.org/obo/bfo.owl#BFO_0000003
bfo:BFO_0000003 rdfs:subClassOf bfo:BFO_0000001 ;
rdfs:label "occurrent"@en-US ;
owl:disjointWith bfo:BFO_0000002 .

# BFO process
###  http://purl.obolibrary.org/obo/bfo.owl#BFO_0000015
bfo:BFO_0000015 rdfs:subClassOf bfo:BFO_0000003 ;
rdfs:label "process"@en-US .

# Introducing Chemical bonds as forces, which are processes and thus occurrents
cg:CG_0001000 rdf:type rdfs:Class ;
		rdfs:subClassOf bfo:BFO_0000015 ;
		rdfs:label "force"@en-US ;
		skos:definition "A force is a process that involves material participants and that influences the participants location and trajectory in space -- either to remain in place or to cause movement or other kinds of spatial changes."@en-US .

# Introducing Chemical bonds as forces, which are processes and thus occurrents
cg:CG_0001001 rdf:type rdfs:Class ;
		rdfs:subClassOf cg:CG_0001000 ;
		rdfs:label "chemical bond"@en-US ;
		skos:definition "A chemical bond is a microscopic force that binds atoms, molecules or subatomic particles together."@en-US .

		


